list5: ex2: finished, ex1,3: sketch

Lista5.v
@@ -1,5 +1,5 @@
 
-Require Import ZArith Wellfounded Wf_nat.
+Require Import ZArith Wellfounded Wf_nat Arith.
 
 
 Section Zad1.
@@ -10,94 +10,152 @@ Section Zad1.
   SearchAbout (Z -> nat).
   Eval compute in Zabs_nat (-4).
 
-  Definition connat x := Zabs_nat (x-c).
-
-  Definition R_c_lt : forall x y , 0 <= c <= x -> R_c x y -> (connat x < connat y )%nat.
+  (* 0 -> 1, neg -> 0, pos -> S pos*)
+  Definition connat x :=
+    match x - c with
+      | 0 => S O
+      | Zneg _ => O
+      | Zpos p => S (nat_of_P p)
+    end.
+(*
+  Lemma connat_inj : forall x y, connat x = connat y -> x -c = y -c.
   Proof.
-    intros.
-    destruct H0.
-    assert (x - c >= 0) by omega.
-    assert (y - c > 0) by omega.
-    unfold connat.
-    assert (x - c < y - c) by omega.
-    apply Zabs_nat_lt.
+    unfold connat;intros; destruct (x-c);destruct(y-c);auto;
+      try discriminate; try omega.
+
+    assert (nat_of_P p > 0)%nat by apply lt_O_nat_of_P.
+    omega.
+
+    assert (nat_of_P p > 0)%nat by apply lt_O_nat_of_P.
+    omega.
+
+    injection H.
+    intro.
+    assert (p = p0) by (apply nat_of_P_inj;auto).
+    congruence.
+
+    admit.
+  Qed.
+
+  Hint Resolve connat_inj.
+
+  Lemma R_c_lt_pos : forall x y , 0 <= x-c < y -c -> (connat x < connat y )%nat.
+  Proof.
+    intros;unfold connat;
+    destruct (x - c);destruct (y - c);try omega.
+
+    assert (nat_of_P p > 0)%nat by apply lt_O_nat_of_P.
+    omega.
+
+    assert (Zneg p < 0) by apply Zlt_neg_0.
+    omega.
+
+    assert (nat_of_P p < nat_of_P p0)%nat.
+      repeat rewrite Zpos_eq_Z_of_nat_o_nat_of_P in *.
+      apply inj_lt_rev.
+      omega.
+    omega.
+
+    assert (Zneg p0 <= Zpos p) by apply Zle_neg_pos.
+    omega.
+
+    assert (Zneg p < 0) by apply Zlt_neg_0.
     omega.
   Qed.
 
-  Hint Resolve R_c_lt.
-  (*
-  Lemma R_c_Acc : forall x, Acc R_c x.
-  Proof.
-    constructor;intros.
-    assert (0 <= c \/ c < 0) by omega.
-    assert (c <= y \/ y < c) by omega.
-    destruct H0.
-    destruct H1.
-    assert (0 <= c <= y) by auto.
-    A
-    rewrite(R_c_lt y x H2);intros.
+  Lemma R_c_lt_neg_pos :forall x y,
+    x  - c < 0 <= y - c -> (connat x < connat y )%nat.
+    intros;unfold connat;
+    assert (x-c < y -c) by omega.
+    destruct (x - c);destruct (y - c);try omega.
 
-    assert
-    induction x;constructor;intros.
-    admit.
-  Qed. *)
+    assert (Zpos p > 0) by apply Zgt_pos_0.
+    omega.
 
-(*  Hint Resolve R_c_Acc.
-  Hint Unfold well_founded. *)
+    assert (nat_of_P p < nat_of_P p0)%nat.
+      repeat rewrite Zpos_eq_Z_of_nat_o_nat_of_P in *.
+      apply inj_lt_rev.
+      omega.
+    omega.
 
+    assert (Zneg p0 <= Zpos p) by apply Zle_neg_pos.
+    omega.
+
+    assert (Zneg p0 < 0) by apply Zlt_neg_0.
+    omega.
+  Qed.
+
+  Hint Resolve R_c_lt_pos R_c_lt_neg_pos.
+*)
   Lemma R_c_wf : well_founded R_c.
   Proof.
     apply well_founded_lt_compat with connat.
     intros.
-    assert (0 <= c \/ c < 0) by omega.
-    assert (c <= x \/ x < c) by omega.
-    destruct H0;destruct H1.
-    assert (0 <= c <= x) by auto.
-    auto.
-
     destruct H.
-    (* x < 0 <= c <= y *)
+    assert (forall p, 0 < nat_of_P p )%nat by
+      apply lt_O_nat_of_P.
+    assert (forall p, Zneg p < 0) by
+      apply Zlt_neg_0 .
+    assert (forall p, 0 < Zpos p) by
+      auto with zarith.
+    unfold connat.
+    assert (x - c < y -c ) by omega.
+    remember (x-c) as xc ;remember (y-c) as yc.
+    destruct yc;destruct xc;try rewrite <- Heqxc, <- Heqyc;
+      try omega; auto with zarith arith.
+    specialize H3 with p; omega.
+    assert (nat_of_P p0 < nat_of_P p)%nat .
+      repeat rewrite Zpos_eq_Z_of_nat_o_nat_of_P in *.
+      apply inj_lt_rev.
+      omega.
+    omega.
+    specialize H2 with p;omega.
     admit.
-    (* x < c < y *)
-
-    elimtype False.
-
+    admit.
+    admit.
     admit.
 
-    elimtype False.
+    simpl.
+
+    auto with zarith.
+    simpl.
+    destruct
+    simpl.
+    destruct H.
+    assert (x - c < y -c) by omega.
+    assert (0 <= x - c  \/ x - c <  0) by omega.
+    destruct H2.
+    assert (0 <= x - c < y -c) by omega.
+    auto.
     admit.
+(*
+    assert (0 <= x - c  \/ x - c <  0) by omega.
+    destruct H3.
+
+    replace (connat x <= connat y)%nat with (connat x < S (connat y))%nat in *.
+  assert (connat x < connat y \/ connat x = connat y)%nat by omega.
+  clear H0.
+  destruct H1.
+  auto.
+  destruct H.
+  assert (x = y).
+    assert (x - c = y - c)  by auto.
+    omega.
+  omega. *)
   Qed.
 
 End Zad1.
 
 Section Zad2.
 
-  Require Import List NArith Ndec.
+  Require Import List NArith Arith.
   Open Scope N_scope.
 
   Notation " [ x ] " := (exist _ x _) : spec_scope.
   Notation " # t " := (proj1_sig t) (at level 60) : spec_scope.
 
   Open Scope spec_scope.
-(*
-  Lemma min_in_nil : forall x, forall y, In y nil -> x <= y.
-    intros.
-    inversion H.
-  Qed.
-  Definition minimum : forall (l:list N), l <> nil ->  { x : N | forall y, In y l -> x <= y }.
-  refine (fun l p =>
-    let fix F x l {struct l}  :=
-      match l with
-        | nil => _ x
-        | y::xs => _ (Nmin y (#(F x xs )))
-      end in
-    match l with
-      | nil => _
-      | x::xs => F x xs
-    end);admit.
-  Defined.
-  apply 0.
-Defined.*)
+
 
   Inductive sorted : list N -> Prop :=
   | sort_nil : sorted nil
@@ -109,15 +167,107 @@ Defined.*)
   decide equality.
   Defined.
 
+  Goal forall x l, sorted (x::l) ->  forall y, In y l -> x <= y.
+    intros.
+    inversion H;subst.
+    destruct H0;subst.
+    auto.
+  Qed.
 
-  Definition insert : forall (x:N), {l | sorted l } -> {l' : list N | sorted l'}.
+  Lemma Nle_trans : forall x y z,
+    x <= y -> y <= z -> x <= z.
+    intros x y z.
+    unfold Nle.
+    repeat rewrite nat_of_Ncompare.
+    repeat rewrite <- nat_compare_le.
+    omega.
+  Qed.
+
+  Lemma sorted_cons : forall x y l,
+    y <= x -> sorted (x::l) -> sorted (y::x::l).
+    intros.
+    constructor;intros;eauto;subst.
+    inversion H0;subst;simpl in*;intuition;eauto;
+    try rewrite <-H2;auto.
+
+    apply Nle_trans with x;auto.
+  Qed.
+  Hint Resolve sorted_cons.
+
+  Lemma sorted_mixin : forall a b c l,
+    sorted (b :: c :: l) -> sorted (a :: b :: l) -> sorted (a :: b :: c:: l).
+    intros.
+    inversion H;simpl;intros;subst.
+    inversion H0;simpl;intros;subst.
+    constructor;intros;auto.
+    simpl in *;intuition.
+    rewrite <- H1.
+    apply Nle_trans with b;intuition.
+  Qed.
+  Hint Resolve sorted_mixin.
+
+  Lemma Nle_refl : forall x, x <= x.
+    intros; unfold Nle.
+    rewrite Ncompare_refl; intros.
+    discriminate.
+  Qed.
+  Hint Resolve Nle_refl.
+
+  Ltac inv_int H :=  inversion H;intros;subst;simpl in *;intuition.
+
+  Lemma sorted_perm : forall x y xs l,
+    y <= x -> sorted (y::xs) -> Permutation (x::xs) l -> sorted l -> sorted (y::l).
+    intros.
+    inv_int H1.
+    constructor;intros;auto.
+    assert (Permutation l (x::xs)) by (apply Permutation_sym;auto).
+    assert (In y0 (x::xs)).
+    apply Permutation_in with l ;auto.
+    inv_int H0; try solve [rewrite <- H8;auto].
+  Qed.
+  Hint Resolve sorted_perm.
+
+  Lemma lt_le : forall x y, x < y -> x <= y.
+    intros.
+    unfold "<=". unfold "<" in H.
+    rewrite H. discriminate.
+  Qed.
+
+  Lemma gt_lt : forall x y, (x ?= y) = Gt -> (y ?= x) = Lt.
+    intros.
+    assert (CompOpp (x ?= y) = (y ?= x)).
+    eauto using Ncompare_antisym.
+    rewrite <- H0.
+    rewrite H.
+    auto.
+  Qed.
+  Hint Constructors Permutation.
+
+  Definition insert : forall (l:list N) (x:N)  ,sorted l  -> {l' : list N | Permutation (x::l) l' /\ sorted l'}.
   refine (
-    fix F x l {struct l} :=
+    fix F l x{struct l} :  sorted l -> {l' : list N | Permutation (x::l) l' /\ sorted l'}  :=
       match l with
-        | exist nil _ => [(x::nil)]
-        | exist (y::xs) p => if le_dec x y then (_ (x::y::xs) p) else ( _ y p (F x)) (*[y::#(F x (_ xs p)) ]*)
-      end) ;eauto.
+        | nil =>  fun _ => _ (x::nil)
+        | y::xs => fun p => if le_dec x y then _ else _ (F xs x _ ) p
+      end);intros.
+  exists (x::nil).
+  intuition;eauto.
+
+  exists (x::y::xs).
+  intuition;eauto.
+
+  destruct x0.
+  assert (y < x) by
+    (apply gt_lt;auto).
+  assert (y <= x) by
+    (apply lt_le;auto).
+
+  exists (y::x0).
+  intuition;eauto.
+
+  inversion p;eauto.
   Defined.
+
 
   Hint Extern 1 =>
     match goal with
@@ -133,35 +283,189 @@ Defined.*)
   constructor;intros;try destruct H;intuition.
   Qed.
 
-  Eval compute in insert 3 (exist _ (1::2::4::nil) s123).
-
-  Definition ins_perm : forall (x:N) l l',
-    Permutation l l' ->  sorted l' ->
-    {lst  : list N | Permutation (x::l) lst /\ sorted lst }.
-
-  refine (fun x l sl => _ (insert x (_ l sl) ));eauto.
-  intros.
-  destruct x0.
-  exists x0.
-  intuition.
-  admit.
-  Qed.
-
-  Hint Resolve ins_perm.
+  Eval compute in insert (1::2::4::nil) 3 s123.
 
   Definition insertsort : forall l : list N,
     {l' : list N | Permutation l l' /\ sorted l'}.
-  refine (fix F (l:list N) : {l' : list N | Permutation l l' /\ sorted l'} :=
-    match  l with
-      | nil => [nil]
-      | x :: xs => (_ x (F xs)) (*ins_perm x xs* (_ (F xs)) (_ (F xs)) (_ (F xs))*)
-    end);eauto.
-  admit.
+  induction l;eauto.
+  destruct IHl.
+  destruct a0.
+  specialize (insert x a H0);intros.
+  destruct H1.
+  exists x0.
+  intuition;eauto.
+  Defined.
+
+  Eval compute in insertsort (2::5::1::6::3::nil).
+End Zad2.
+
+Section Zad3.
+  Parameter A : Type.
+
+  Section ListT.
+    Inductive listT :=
+    | nilT  : listT
+    | consT : A -> listT -> listT.
+  End ListT.
+
+  Definition index := nat.
+
+  Inductive expr : Set :=
+  | Atom : index -> expr
+  | Plus : expr -> expr -> expr .
+
+  Definition atommap := list nat.
+
+  Definition interp_var (i:index) (vm:atommap) := nth i vm  0.
+
+  Fixpoint interp vm e  :=
+    match e with
+      | Atom i => interp_var i vm
+      | Plus e1 e2 => interp vm e1  + interp vm e2
+    end.
+
+  Fixpoint flat_expr_aux e acc :=
+    match e with
+      | Atom i => Plus e acc
+      | Plus e1 e2 => flat_expr_aux e1 (flat_expr_aux e2 acc)
+    end.
+
+  Fixpoint flat_expr e :=
+    match e with
+      | Atom _ => e
+      | Plus e1 e2 => flat_expr_aux e1 (flat_expr e2)
+    end.
+
+  Lemma flat_aux_correct : forall vm e1 e2,
+    interp vm e1 + interp vm e2 = interp vm (flat_expr_aux e1 e2).
+    double induction e1 e2;intros;simpl;
+    repeat match goal with
+             | [ H : context [ _ = interp _ ( flat_expr_aux _ _)] |- _ ] => rewrite <- H
+           end;simpl;auto with arith.
   Qed.
 
+  Hint Rewrite <- flat_aux_correct : db .
+  Lemma flat_correct : forall vm e1 e2,
+    interp vm (flat_expr e1) = interp vm (flat_expr e2)
+    -> interp vm e1 = interp vm e2.
+    assert (forall vm e, interp vm e = interp vm (flat_expr e)) by
+      (induction e; simpl; try autorewrite with db; auto).
+    intros; do 2 rewrite <- H in *;trivial.
+  Qed.
+
+  Lemma interp_rev_corr : forall vm e,
+    interp vm e = interp (rev vm) e.
+    induction e;intros;simpl.
+    admit.
+
+    rewrite IHe1, IHe2;auto.
+  Qed.
+  Hint Rewrite <- interp_rev_corr : db.
+
+  Lemma interp_rev_refl : forall vm e1 e2,
+    interp (rev vm) e1 = interp (rev vm) e2
+    -> interp vm e1 = interp vm e2.
+    intros.
+    autorewrite with db in H.
+    auto.
+  Qed.
+
+  Fixpoint listT_to_atommap (lst : list nat) :=
+    match lst with
+      | nil => fun _ => 0
+      | a :: xs => fun n =>
+        match n with
+          | 0 => a
+          | S m => listT_to_atommap xs m
+        end
+    end.
+
+
+  Ltac insert_atom atoms a :=
+    match atoms with
+      | nil => constr:(a::nil)
+      | a ::  _ => atoms
+      | ?x :: ?xs =>
+        let ys := insert_atom xs a in
+          constr:(x ::ys)
+    end.
+
+  Ltac enum_atoms atoms a :=
+    match a with
+      | ?e1 + ?e2 => enum_atoms ltac:(enum_atoms atoms e1) e2
+      | _ => insert_atom atoms a
+    end.
+
+  Ltac enum_atom a  := enum_atoms (@nil nat) a.
+
+  Ltac find_atom a lst :=
+    match lst with
+      | a ::  _ => constr: 0
+      |  _ :: ?xs =>
+        let n := find_atom a xs in
+          constr: (S n)
+    end.
+
+  Ltac model atoms v :=
+    match v with
+      | (?X1 + ?X2) =>
+        let r1 := model atoms X1 with r2 := model atoms X2
+          in constr : (Plus r1 r2)
+      | _  =>
+        let n := find_atom v atoms in
+          constr: (Atom n)
+    end.
+
+
+  Ltac prover :=
+    intros;
+    match goal with
+      | [ |- ?X1 = ?X2] =>
+        let atoms1 := enum_atom X1 in
+        let atoms2 := enum_atom X2 in
+          let e1 := model atoms1 X1 in
+          let e2 := model atoms2 X2 in
+            (change (interp atoms1 e1 =
+                     interp atoms2 e2)
+            ; repeat (apply flat_correct || apply interp_rev_corr ); reflexivity)
+      | _ => idtac "dupa"
+    end.
+
+  Definition nmn := Plus (Atom 0) (Plus (Atom 1) (Atom 0)).
+  Definition mnn := Plus (Atom 0) (Plus (Atom 1) (Atom 1)).
+  Lemma refl_test : forall n m,
+    n+(m+n) = m+(n+n).
+    intros.
+    change (interp (n::m::nil) nmn = interp (m::n::nil) mnn).
+    unfold nmn,mnn.
+    rewrite interp_rev_corr.
+    simpl rev.
+    apply flat_correct.
+    change (interp (n::m::nil) (Plus (Atom 0) (Plus (Atom 1) )) = interp (y::x::nil) (Plus (Atom 0) (Atom 1))).
+    prover.
+    intros.
+    change (interp (x::y::nil) (Plus (Atom 0) (Atom 1)) = interp (y::x::nil) (Plus (Atom 0) (Atom 1))).
+    apply interp_rev_corr.
+    rewrite interp_rev_corr.
+    simpl.
+    auto.
+    reflexivity.
+    auto.
+    prover.
   admit.
-  intros.
-  intros.
-  admit.
-  intros.
-  destruct x1.
+  Qed.
+  Lemma refl_test2 : forall x y z,
+    x + y + z = x + (y + z).
+    prover.
+  Qed.
+  Lemma reflection_test_norm : forall f x y z t u,
+    (f x + x) + (1 + y + z + (t + u)) = f x + x + 1 + y + (z + (t + u)).
+  Proof.
+    prover.
+  Qed.
+
+
+
+
+
+End Zad3.
